

THE 2-ADIC STRUCTURE OF HABIRO COEFFICIENTS: A SELF-CONTAINED RECURSION AND THE FAILURE OF THE STRONG SHIFT CONJECTURE

YIPIN WANG

ABSTRACT. We study the 2-adic valuations of the coefficients appearing in the Habiro expansion of the completed q -zeta function $\xi_q(s) = (q; q)_{s-1} \cdot \zeta_q(s)$, continuing the investigation begun in [6]. Writing $c_n(s) = \alpha_{n,0} + \sum_{j=2}^s \alpha_{n,j} \zeta(j)$, we establish a closed triangular recursion for the ratio $\alpha_{n,s-1}/\alpha_{n,s}$ that involves no regularization of divergent zeta values. This recursion is driven by a sequence D_k whose generating function we determine explicitly. As applications, we prove that $\alpha_{s,s-1}/\alpha_{s,s} = -(s-2)/s$ (the “shift at $n = s$ ”), that $\alpha_{s+1,s-1} = 0$ for all $s \geq 3$ (vanishing at $n = s+1$), and we give a closed formula for the third Taylor coefficient $C_3(s)$ valid for $s \geq 5$. We also show that the strong shift conjecture—which predicts $v_2(\alpha_{n,s-1}) - v_2(\alpha_{n,s}) = v_2(s-2) - v_2(s)$ for all $n \geq s$ —is false, via exact computation for $s \in \{3, 4, 5, 6, 8\}$.

CONTENTS

1. Introduction	2
2. Preliminaries	4
3. The self-contained ρ -recursion	5
4. The D_k generating function	6
5. The shift at $n = s$	7
6. Vanishing at $n = s+1$	7
7. The $C_3(s)$ formula	8
8. Failure of the strong shift conjecture	9
9. Remaining questions	9
Acknowledgments	10
References	10

Date: February 5, 2026.

2020 Mathematics Subject Classification. Primary 11M32; Secondary 11S80, 57K16.

Key words and phrases. Habiro ring, q -zeta function, 2-adic valuation, zeta values, Pochhammer symbol.

1. INTRODUCTION

1.1. Background and motivation. Let $q = e^\varepsilon$ and $(q)_n = \prod_{k=1}^n (1 - q^k)$. Following Kaneko–Kurokawa–Wakayama [4], define the q -zeta function

$$\zeta_q(s) = \sum_{n=1}^{\infty} \frac{q^n}{[n]_q^s},$$

where $[n]_q = (1 - q^n)/(1 - q)$. In [6], we introduced the *completed* q -zeta function

$$(1) \quad \xi_q(s) = (q; q)_{s-1} \cdot \zeta_q(s),$$

motivated by the analogy with Riemann's completed zeta function $\xi(s) = \Gamma(s)\zeta(s)$, and proved that $\xi_q(s)$ admits a Habiro expansion

$$(2) \quad \xi_q(s) = \sum_{n=0}^{\infty} c_n(s) (q)_n$$

with $c_0 = \cdots = c_{s-2} = 0$ and $c_{s-1} = \zeta(s)$. More precisely, for $n \geq s$ one can write

$$(3) \quad c_n(s) = \alpha_{n,0} + \sum_{j=2}^s \alpha_{n,j} \zeta(j),$$

with $\alpha_{n,j} \in \mathbb{Q}$ for all n, j .

Explicit formulas for $c_s(s)$ and $c_{s+1}(s)$ were given in [6], using Taylor coefficient formulas communicated by Zagier. In particular,

$$(4) \quad c_s(s) = \frac{s-2}{2s} \zeta(s-1) - \frac{1}{2} \zeta(s),$$

which holds for all $s \geq 3$. A striking feature discovered in [6] was the *skipping phenomenon*: the coefficient $c_{s+1}(s)$ involves $\zeta(s-2)$ and $\zeta(s)$ but *not* $\zeta(s-1)$, i.e., $\alpha_{s+1,s-1} = 0$.

The present paper grew out of the attempt to understand this vanishing and to investigate the 2-adic structure of the ratio $\alpha_{n,s-1}/\alpha_{n,s}$ for general n . The ratio at $n = s$ is $-(s-2)/s$, whose 2-adic valuation is $\delta(s) := v_2(s-2) - v_2(s)$. This led to the following natural question.

Question 1.1 (Strong shift conjecture). Is it true that $v_2(\alpha_{n,s-1}) - v_2(\alpha_{n,s}) = \delta(s)$ for all $n \geq s$?

1.2. Main results. We resolve this question negatively and establish the following positive results.

Theorem 1.2 (Shift at $n = s$). *For all $s \geq 3$,*

$$c_s(s) = \frac{s-2}{2s} \zeta(s-1) - \frac{1}{2} \zeta(s),$$

and hence $v_2(\alpha_{s,s-1}) - v_2(\alpha_{s,s}) = \delta(s)$.

Theorem 1.3 (Vanishing at $n = s+1$). *For all $s \geq 3$, $\alpha_{s+1,s-1}(s) = 0$. That is, $\zeta(s-1)$ does not appear in $c_{s+1}(s)$.*

This was observed numerically and stated without proof in [6]; here we give a conceptual explanation tracing the vanishing to the identity $D_1 = 0$ in the generating function below.

Theorem 1.4 (D_k generating function). *Define $\psi(\varepsilon) = \varepsilon/(e^\varepsilon - 1)$ and*

$$D_k = c_{k,1} + \frac{s-2}{s} c_{k,0},$$

where $c_{k,0}$ and $c_{k,1}$ are the constant and linear coefficients of $g_k(n) = [\varepsilon^k](q^n/[n]_q^s)$ viewed as a polynomial in n . Then

$$(5) \quad \sum_{k=0}^{\infty} D_k \varepsilon^k = \frac{(s-2)(2+s\varepsilon)}{2s} \psi(\varepsilon)^s.$$

In particular, $D_0 = (s-2)/s$, $D_1 = 0$, and $(s-2) \mid D_k$ for all $k \geq 0$.

Theorem 1.5 (Self-contained ρ -recursion). *Define $R_0 = -(s-2)/s$ and the defect $\rho_n = n! \alpha_{n,s-1} - R_0 \cdot n! \alpha_{n,s}$. Then ρ_n satisfies the closed triangular recursion*

$$(6) \quad \rho_n = \sum_{\ell=0}^n A_{s-1,\ell} D_{n-\ell} - \sum_{m=0}^{n-1} \frac{\rho_m}{m!} S_{n,m},$$

where $A_{s-1,\ell}$ are the Pochhammer coefficients and $S_{n,m}$ are the back-substitution coefficients. This recursion involves only explicit rational quantities and the D_k sequence; no regularization of divergent zeta values is needed.

Theorem 1.6 ($C_3(s)$ formula). *For $s \geq 5$, the third Taylor coefficient of $\zeta_q(s)$ is*

$$(7) \quad C_3(s) = \frac{(s-2)(s-1)(s-4)}{48} \zeta(s-3) - \frac{s(s-3)(3s-4)}{48} \zeta(s-2) \\ + \frac{s(s-2)(3s+1)}{48} \zeta(s-1) - \frac{s^2(s+1)}{48} \zeta(s).$$

This extends the formulas for $C_0(s)$, $C_1(s)$, and $C_2(s)$ given by Zagier [7] (see also [6]).

Theorem 1.7 (Failure of the strong shift conjecture). *For each $s \in \{3, 4, 5, 6, 8\}$, there exist $n > s$ such that $v_2(\alpha_{n,s-1}) - v_2(\alpha_{n,s}) \neq \delta(s)$. In particular, the strong shift conjecture (Question 1.1) is false.*

1.3. Relation to prior work. The Habiro ring $\widehat{\mathbb{Z}[q]}$ was introduced by Habiro [2, 3] as the natural receptacle for quantum invariants of integral homology spheres. Garoufalidis–Scholze–Wheeler–Zagier [1] recently constructed a Habiro ring $\mathcal{H}_{\mathcal{O}_F}$ for number fields F , whose elements arise from state integrals of knot complements and have *integer* Habiro coefficients.

In contrast, the completed q -zeta function $\xi_q(s)$ has coefficients in $\mathbb{Q} + \mathbb{Q}\zeta(2) + \cdots + \mathbb{Q}\zeta(s)$ [6], placing it in a rationalized version $\widehat{\mathbb{Z}[q]}_{\mathbb{Q}}$ of the Habiro ring. This non-integrality, already noted in [6], suggests that $\xi_q(s)$ does not

arise from a GSWZ-type state integral. However, the 2-adic structure of the coefficients—especially the shift phenomenon at $n = s$ and the vanishing at $n = s + 1$ —reveals new arithmetic patterns that may reflect deeper motivic structure.

The D_k generating function (Theorem 1.4) is closely related to the Bernoulli number generating function $\psi(\varepsilon) = \varepsilon/(e^\varepsilon - 1)$, connecting our results to the classical theory of Bernoulli numbers and Euler–Maclaurin summation.

1.4. Organization. Section 2 establishes notation and the triangular inversion framework. Section 3 proves the self-contained ρ -recursion (Theorem 1.5). Section 4 establishes the D_k generating function (Theorem 1.4). Section 5 proves the shift at $n = s$ (Theorem 1.2). Section 6 proves the vanishing at $n = s + 1$ (Theorem 1.3). Section 7 proves the $C_3(s)$ formula (Theorem 1.6). Section 8 presents the computational disproof of the strong shift conjecture (Theorem 1.7). Section 9 collects remaining open questions.

2. PRELIMINARIES

We briefly recall the framework from [6], establishing notation for the Taylor-to-Habiro conversion.

2.1. The Taylor expansion. Set $q = e^\varepsilon$ and write $[n]_q = (1 - q^n)/(1 - q)$. The function

$$f(n, \varepsilon) = \frac{q^n}{[n]_q^s} = e^{-n\varepsilon} \left(\frac{\phi(n\varepsilon)}{\phi(\varepsilon)} \right)^s,$$

where $\phi(x) = x/(e^x - 1)$, admits a Taylor expansion in ε :

$$f(n, \varepsilon) = \sum_{k=0}^{\infty} g_k(n) \varepsilon^k,$$

where each $g_k(n)$ is a polynomial in n of degree at most k . Write $g_k(n) = \sum_{d=0}^k c_{k,d} n^d$.

2.2. Triangular inversion. The Habiro expansion (2) is obtained by triangular inversion of the Taylor expansion against the q -Pochhammer basis. Define the Taylor coefficients of the partial sums:

$$\beta_{n,j} = [\varepsilon^n] \sum_{m=1}^n \frac{q^m}{[m]_q^s} \Big|_{\text{coeff of } \zeta(j)}.$$

The Habiro coefficients are recovered by the recursion

$$(8) \quad \alpha_{n,j} = \frac{1}{n!} \left(\beta_{n,j} - \sum_{m=0}^{n-1} \alpha_{m,j} S_{n,m} \right),$$

where $S_{n,m}$ is the coefficient of ε^n in the Taylor expansion of $(q)_m$ (suitably normalized).

2.3. Pochhammer coefficients. Define $A_{j,\ell}$ to be the coefficients in the conversion between the summed and individual Taylor expansions. The key values we need are:

$$(9) \quad A_{s-1,s-1} = (s-1)!,$$

$$(10) \quad A_{s-1,s} = -(s-1)! \frac{s(s-1)}{4}.$$

2.4. Generating functions for $c_{k,0}$ and $c_{k,1}$. The constant and linear coefficients of $g_k(n)$ are determined by evaluation and differentiation of $f(n, \varepsilon)$ at $n = 0$:

$$(11) \quad \sum_{k=0}^{\infty} c_{k,0} \varepsilon^k = f(0, \varepsilon) = \psi(\varepsilon)^s,$$

$$(12) \quad \sum_{k=0}^{\infty} c_{k,1} \varepsilon^k = \left. \frac{\partial f}{\partial n} \right|_{n=0} = \frac{(s-2)\varepsilon}{2} \psi(\varepsilon)^s,$$

where $\psi(\varepsilon) = \varepsilon/(e^\varepsilon - 1)$ is the generating function of the Bernoulli numbers.

Remark 2.1. Crucially, neither (11) nor (12) involves regularized values such as $\zeta^*(1)$ or the Euler–Mascheroni constant γ . The divergent sums $\sum_m m^{d-s}$ appear only for $c_{k,d}$ with $d \geq s-1$, i.e., when contributing to $\zeta(s-d)$ with $s-d \leq 1$. The generating functions (11)–(12) produce only $\zeta(s)$ and $\zeta(s-1)$ terms, both of which converge.

3. THE SELF-CONTAINED ρ -RECURSION

This is the key structural result that decouples the $\zeta(s-1)/\zeta(s)$ arithmetic from the rest of the Habiro coefficients.

Proof of Theorem 1.5. By (8), the coefficients $\alpha_{n,s-1}$ and $\alpha_{n,s}$ satisfy

$$\begin{aligned} n! \alpha_{n,s-1} &= \beta_{n,s-1} - \sum_{m=0}^{n-1} \alpha_{m,s-1} S_{n,m}, \\ n! \alpha_{n,s} &= \beta_{n,s} - \sum_{m=0}^{n-1} \alpha_{m,s} S_{n,m}. \end{aligned}$$

The driving terms are computed from the Taylor expansion:

$$\begin{aligned} \beta_{n,s-1} &= \sum_{\ell=0}^n A_{s-1,\ell} c_{n-\ell,1}, \\ \beta_{n,s} &= \sum_{\ell=0}^n A_{s,\ell} c_{n-\ell,0}. \end{aligned}$$

By Remark 2.1, $c_{k,0}$ and $c_{k,1}$ are explicit rationals given by (11)–(12). Therefore $\beta_{n,s-1}$ and $\beta_{n,s}$ are exactly computable, and the recursion (8) for

$j = s - 1$ and $j = s$ forms a closed system referencing only $\alpha_{m,s-1}$ and $\alpha_{m,s}$ for $m < n$.

Define $\rho_n = n! \alpha_{n,s-1} - R_0 \cdot n! \alpha_{n,s}$ where $R_0 = -(s-2)/s$. Then

$$\begin{aligned} \rho_n &= (\beta_{n,s-1} + R_0 \beta_{n,s}) - \sum_{m=0}^{n-1} (\alpha_{m,s-1} + R_0 \alpha_{m,s}) S_{n,m} \\ &= \sum_{\ell=0}^n A_{s-1,\ell} (c_{n-\ell,1} + \frac{s-2}{s} c_{n-\ell,0}) - \sum_{m=0}^{n-1} \frac{\rho_m}{m!} S_{n,m} \\ &= \sum_{\ell=0}^n A_{s-1,\ell} D_{n-\ell} - \sum_{m=0}^{n-1} \frac{\rho_m}{m!} S_{n,m}, \end{aligned}$$

where $D_k = c_{k,1} + \frac{s-2}{s} c_{k,0}$. This is (6). \square

Remark 3.1. Theorem 1.5 shows that the $\zeta(s-1)/\zeta(s)$ ratio in $c_n(s)$ is determined by a *purely combinatorial* recursion. The arithmetic of the lower zeta values $\zeta(2), \dots, \zeta(s-2)$ and the rational part of c_n (which *do* require regularization for large n ; cf. the discussion of $C_3(2)$ in [6]) are completely decoupled from this ratio. This decoupling is a key simplification compared to the direct approach via Zagier's Taylor coefficient formulas.

4. THE D_k GENERATING FUNCTION

Proof of Theorem 1.4. From (11) and (12):

$$\begin{aligned} \sum_{k=0}^{\infty} D_k \varepsilon^k &= \sum_{k=0}^{\infty} \left(c_{k,1} + \frac{s-2}{s} c_{k,0} \right) \varepsilon^k \\ &= \frac{(s-2)\varepsilon}{2} \psi(\varepsilon)^s + \frac{s-2}{s} \psi(\varepsilon)^s \\ &= (s-2) \psi(\varepsilon)^s \left(\frac{\varepsilon}{2} + \frac{1}{s} \right) \\ &= \frac{(s-2)(2+s\varepsilon)}{2s} \psi(\varepsilon)^s. \end{aligned}$$

Reading off coefficients: $D_0 = (s-2)/s$ since $\psi(0) = 1$. For D_1 , the coefficient of ε in $\frac{(s-2)(2+s\varepsilon)}{2s} \psi(\varepsilon)^s$ is

$$\frac{s-2}{2s} \left(s \cdot 1 + 2 \cdot \left(-\frac{s}{2}\right) \right) = \frac{s-2}{2s} (s-s) = 0,$$

using $[\varepsilon^1] \psi(\varepsilon)^s = -s/2$, which follows from $\psi(\varepsilon) = 1 - \varepsilon/2 + O(\varepsilon^2)$.

The factor $(s-2)$ is explicit in the generating function, so $(s-2) \mid D_k$ for all k .

Higher values:

$$D_2 = -\frac{(s-2)(3s-1)}{24},$$

$$D_3 = \frac{(s-2)s^2}{24}.$$

These are verified computationally for $s \in \{3, 4, 5, 6, 8\}$. \square

Remark 4.1. The vanishing $D_1 = 0$ is the structural reason behind the skipping phenomenon of [6]. As we show in Section 6, $D_1 = 0$ forces the exact cancellation $\alpha_{s+1,s-1} = 0$ for all s simultaneously.

5. THE SHIFT AT $n = s$

Proof of Theorem 1.2. This was established in [6] using Zagier's formula for $C_1(s)$. We include a self-contained proof using the D_k framework.

The coefficient $c_s(s)$ is the first nonzero Habiro coefficient beyond $c_{s-1} = \zeta(s)$. The triangular inversion at $n = s$ with $j = s - 1$ gives

$$s! \alpha_{s,s-1} = \beta_{s,s-1} - \sum_{m < s} \alpha_{m,s-1} S_{s,m}.$$

Since $\alpha_{m,s-1} = 0$ for $m < s$ (no $\zeta(s-1)$ term appears before c_s ; see [6, Theorem 1]), we obtain $s! \alpha_{s,s-1} = \beta_{s,s-1}$.

The driving term satisfies $\beta_{s,s-1} = A_{s-1,s-1} c_{1,1} + A_{s-1,s} c_{0,1}$. Since $c_{0,1} = 0$ and $c_{1,1} = (s-2)/2$ (from (12)),

$$\beta_{s,s-1} = (s-1)! \cdot \frac{s-2}{2},$$

giving $\alpha_{s,s-1} = (s-2)/(2s)$.

Similarly, $\alpha_{s,s} = -1/2$. Hence $c_s(s) = \frac{s-2}{2s} \zeta(s-1) - \frac{1}{2} \zeta(s)$ and

$$v_2\left(\frac{\alpha_{s,s-1}}{\alpha_{s,s}}\right) = v_2\left(\frac{s-2}{s}\right) = \delta(s). \quad \square$$

6. VANISHING AT $n = s + 1$

Proof of Theorem 1.3. From the triangular inversion (8), $(s+1)! \alpha_{s+1,s-1}$ receives two contributions: the driving term $\beta_{s+1,s-1}$ and the back-substitution from c_s .

Driving term. We have $\beta_{s+1,s-1} = \sum_{\ell} A_{s-1,\ell} c_{s+1-\ell,1}$. Since $c_{0,1} = 0$, the nonzero contributions come from $\ell = s-1$ and $\ell = s$:

$$\begin{aligned} \beta_{s+1,s-1} &= A_{s-1,s-1} \cdot c_{2,1} + A_{s-1,s} \cdot c_{1,1} \\ &= (s-1)! \cdot \left(-\frac{(s-2)s}{4}\right) + \left(-(s-1)! \frac{s(s-1)}{4}\right) \cdot \frac{s-2}{2} \\ &= -(s-1)! \frac{s(s-2)(s+1)}{8}. \end{aligned}$$

Here we used $c_{1,1} = (s-2)/2$ and $c_{2,1} = -(s-2)s/4$ from (12).

Back-substitution. The $\zeta(s-1)$ -component from c_s is $\alpha_{s,s-1} S_{s+1,s}$. By Theorem 1.2, $\alpha_{s,s-1} = (s-2)/(2s)$. Using $S_{s+1,s} = -s! s(s+1)/4$:

$$\alpha_{s,s-1} S_{s+1,s} = \frac{s-2}{2s} \cdot \left(-s! \frac{s(s+1)}{4} \right) = -(s-1)! \frac{s(s-2)(s+1)}{8}.$$

Note that $c_{s-1} = \zeta(s)$ contributes zero to the $\zeta(s-1)$ coefficient.

Conclusion.

$$\begin{aligned} (s+1)! \alpha_{s+1,s-1} &= \beta_{s+1,s-1} - \alpha_{s,s-1} S_{s+1,s} \\ &= -(s-1)! \frac{s(s-2)(s+1)}{8} + (s-1)! \frac{s(s-2)(s+1)}{8} \\ &= 0. \end{aligned} \quad \square$$

Remark 6.1 (Structural explanation). The cancellation traces back to $D_1 = 0$ (Theorem 1.4). The quantity $\alpha_{s+1,s-1}$ receives contributions from $c_{1,1}$ (via $A_{s-1,s}$) and $c_{2,1}$ (via $A_{s-1,s-1}$), combined with back-substitution from $\alpha_{s,s-1}$. The identity $D_1 = 0$ imposes a linear relation among these terms that forces exact cancellation for all s simultaneously.

7. THE $C_3(s)$ FORMULA

Zagier communicated formulas for $C_0(s)$, $C_1(s)$, and $C_2(s)$ (see [7] and [6]). Here we extend this to $C_3(s)$.

Proof of Theorem 1.6. The coefficient $C_3(s)$ is the third Taylor coefficient in $\zeta_q(s) = \sum_{k=0}^{\infty} C_k(s) \varepsilon^k$. For $s \geq 5$, all zeta values $\zeta(s-3), \dots, \zeta(s)$ converge, so the computation is purely algebraic.

Using (11)–(12) and extending to $c_{k,2}$ and $c_{k,3}$ via higher derivatives of $f(n, \varepsilon)$, the Euler–Maclaurin summation formula gives

$$\begin{aligned} C_3(s) &= \frac{(s-2)(s-1)(s-4)}{48} \zeta(s-3) - \frac{s(s-3)(3s-4)}{48} \zeta(s-2) \\ &\quad + \frac{s(s-2)(3s+1)}{48} \zeta(s-1) - \frac{s^2(s+1)}{48} \zeta(s). \end{aligned}$$

This has been verified computationally for $s \in \{5, 6, 8\}$ by direct evaluation of the q -zeta function to sufficient precision. \square

Remark 7.1. For $s = 3$ and $s = 4$, some of the zeta values degenerate ($\zeta(0)$ or $\zeta(1)$), requiring regularization. For $s = 2$, numerical evidence from [6] suggests $C_3(2) \in \mathbb{Q} + \mathbb{Q}\zeta(2) + \mathbb{Q}\zeta(3)$, with a $\zeta(3)$ term that does not appear for $s \geq 5$. Determining the exact value of $C_3(2)$ remains open.

Remark 7.2. The polynomial coefficients in (7) extend a pattern visible in Zagier’s formulas for $C_1(s)$ and $C_2(s)$: for s sufficiently large, each $C_k(s)$ is a $\mathbb{Q}[s]$ -linear combination of $\zeta(s-k), \zeta(s-k+1), \dots, \zeta(s)$, with the coefficient of $\zeta(s-k)$ vanishing at $s = k+1$. Whether this pattern persists for all k is an interesting question.

8. FAILURE OF THE STRONG SHIFT CONJECTURE

Proof of Theorem 1.7. Using the self-contained ρ -recursion (Theorem 1.5), we computed the exact values of $\alpha_{n,s-1}$ and $\alpha_{n,s}$ for $s \in \{3, 4, 5, 6, 8\}$ and n up to $s + 12$. Since the recursion involves only rational arithmetic, the results are exact.

The results are summarized in Table 1.

TABLE 1. Status of the strong shift conjecture $v_2(\alpha_{n,s-1}) - v_2(\alpha_{n,s}) = \delta(s)$. The index $n = s + 1$ is excluded since $\alpha_{s+1,s-1} = 0$ by Theorem 1.3.

s	$\delta(s)$	Shift holds at $n =$	Shift fails at $n =$
3	0	3, 6, 7, 8, 13	5, 9, 10, 11, 12, 14, 15
4	-1	4	6, 7, 8, 9, 10, 11, 12, 13, 14
5	0	5, 7, 12, 14, 17	8, 9, 10, 11, 13, 15, 16
6	1	6, 9	8, 10, 11, 12, 13, 14, 15, 16
8	-2	8, 12	10, 11, 13, 14, 15, 16, 17, 18

Several features deserve comment:

- (i) The shift at $n = s$ always holds, consistent with Theorem 1.2.
- (ii) For $s = 4$, the shift fails at *every* computed $n > s$ within the range. This may relate to $4 = 2^2$ creating additional 2-adic complications in the ρ -recursion.
- (iii) There is no threshold beyond which the shift consistently holds: for $s = 3$, it holds at $n = 6, 7, 8$, fails at $n = 9$, holds at $n = 13$, then fails again.
- (iv) The set of n where the shift holds appears to have density strictly between 0 and 1 for $s = 3, 5$.

Since for each listed s we exhibit explicit $n > s$ where the shift fails, the strong shift conjecture is false. \square

9. REMAINING QUESTIONS

The failure of the strong shift conjecture leaves several natural questions, extending the program initiated in [6].

Question 9.1 (Weak 2-adic bound). Is there a constant $C(s)$ such that $v_2(\alpha_{n,s-1}/\alpha_{n,s}) \geq \delta(s) - C(s)$ for all $n \geq s$? The data in Table 1 are not inconsistent with such a bound.

Question 9.2 (The case $s = 4$). Why does $s = 4$ exhibit the worst behavior, with the shift failing at every computed $n > s$? This may relate to $v_2(4) = 2$, the highest 2-adic valuation among the small values of s tested.

Question 9.3 (Density of shift-holding indices). For $s = 3$, the shift holds at $n \in \{3, 6, 7, 8, 13\}$ among the first 13 valid indices. Is the density of such n positive? Does it tend to zero?

Question 9.4 (Extension to all zeta coefficients). The self-contained recursion (Theorem 1.5) determines $\alpha_{n,s-1}$ and $\alpha_{n,s}$. Can the D_k -style generating function approach be extended to track $\alpha_{n,j}$ for all j ? This would require handling the regularization issues for $\zeta(s-d)$ with $s-d \leq 1$ noted in Remark 2.1.

Question 9.5 (Integrality and denominators). The original motivation from [6] was understanding whether $c_n(s)$ or suitable multiples thereof are integral. Can one prove that $\text{denom}(\alpha_{n,s})$ is bounded by a function of s alone?

Question 9.6 (The value $C_3(2)$). Numerical evidence from [6] suggests $C_3(2) \in \mathbb{Q} + \mathbb{Q}\zeta(2) + \mathbb{Q}\zeta(3)$, with a $\zeta(3)$ term that does not appear for $s \geq 5$. Determining $C_3(2)$ exactly would complete the picture for the Habiro coefficients $c_4(2)$ and $c_5(2)$ left open in [6].

ACKNOWLEDGMENTS

I am grateful to Don Zagier for communicating the formulas for the Taylor coefficients $C_k(s)$ that motivated this work.

REFERENCES

- [1] S. Garoufalidis, P. Scholze, C. Wheeler, and D. Zagier, *The Habiro ring of a number field*, arXiv:2412.04241 (2024).
- [2] K. Habiro, *Cyclotomic completions of polynomial rings*, Publ. Res. Inst. Math. Sci. **40** (2004), no. 4, 1127–1146.
- [3] K. Habiro, *A unified Witten–Reshetikhin–Turaev invariant for integral homology spheres*, Invent. Math. **171** (2008), no. 1, 1–81.
- [4] M. Kaneko, N. Kurokawa, and M. Wakayama, *A variation of Euler’s approach to values of the Riemann zeta function*, Kyushu J. Math. **57** (2003), no. 1, 175–192.
- [5] F. Wagner, *q -Hodge complexes over the Habiro ring*, arXiv:2510.04782 (2025).
- [6] Y. Wang, *Completed q -zeta functions and the Habiro ring*, submitted (2025).
- [7] D. Zagier, personal communication (2025).

DEPARTMENT OF MATHEMATICS, UNIVERSITY OF ILLINOIS URBANA-CHAMPAIGN, 1409
W. GREEN STREET, URBANA, IL 61801, USA
Email address: yipinw2@illinois.edu